minor refac

Computability/RecursiveInTheorems.lean
@@ -1,58 +1,98 @@
 import Computability.Encoding
 import Mathlib.Data.PFun
-
 import Mathlib.Data.Nat.Dist
 
-open Computability
 open Classical
 open Nat.RecursiveIn.Code
 
-variable {α : Type*} {β : Type*} {σ : Type*}
+variable {α:Type*} {β:Type*} {σ:Type*}
 variable [Primcodable α] [Primcodable β] [Primcodable σ]
 
 -- conversions between oracle and non-oracle versions
-lemma PrimrecIn.PrimrecIn_Empty (h : Nat.PrimrecIn (fun _=>0) f) : Nat.Primrec f := by
+lemma PrimrecIn.PrimrecIn_Empty (h:Nat.PrimrecIn (fun _=>0) f):Nat.Primrec f := by
   induction' h with g hg g h _ _ ih₁ ih₂ g h _ _ ih₁ ih₂ g h _ _ ih₁ ih₂ g _ ih
   repeat {constructor}
   · (expose_names; exact Nat.Primrec.pair a_ih a_ih_1)
   repeat {constructor; assumption; try assumption}
   (expose_names; exact Nat.Primrec.prec a_ih a_ih_1)
-lemma PrimrecIn.PrimrecIn₂_Empty {f:α→β→σ} (h : PrimrecIn₂ (fun _=>0) f) : Primrec₂ f := by
+lemma PrimrecIn.PrimrecIn₂_Empty {f:α→β→σ} (h:PrimrecIn₂ (fun _=>0) f):Primrec₂ f := by
   unfold PrimrecIn₂ at h
   unfold Primrec₂
   apply PrimrecIn.PrimrecIn_Empty
   exact h
-
-theorem Primrec.to_PrimrecIn₂ {f:α→β→σ} (h : Primrec₂ f) : PrimrecIn₂ O f := by
+theorem Primrec.to_PrimrecIn₂ {f:α→β→σ} (h:Primrec₂ f):PrimrecIn₂ O f := by
   unfold Primrec₂ at h
   unfold PrimrecIn₂
   apply Primrec.to_PrimrecIn
   exact h
-
-theorem PrimrecIn.PrimrecIn₂_iff_Primrec₂ {f:α→β→σ} : (∀O,PrimrecIn₂ O f) ↔ Primrec₂ f := by
+theorem PrimrecIn.PrimrecIn₂_iff_Primrec₂ {f:α→β→σ}:(∀O,PrimrecIn₂ O f) ↔ Primrec₂ f := by
   constructor
   · exact fun a ↦ PrimrecIn₂_Empty (a fun x ↦ 0)
   · exact fun a O ↦ Primrec.to_PrimrecIn₂ a
-theorem PrimrecIn.PrimrecIn_iff_Primrec : (∀O,Nat.PrimrecIn O f) ↔ Nat.Primrec f := by
+theorem PrimrecIn.PrimrecIn_iff_Primrec:(∀O,Nat.PrimrecIn O f) ↔ Nat.Primrec f := by
   constructor
   · exact fun a ↦ PrimrecIn.PrimrecIn_Empty (a fun x ↦ 0)
   · exact fun a O ↦ Nat.Primrec.to_PrimrecIn a
 
+-- instance Code : Primcodable (Nat.RecursiveIn.Code) := by exact Primcodable.ofDenumerable Nat.RecursiveIn.Code
+namespace Nat.RecursiveIn.Code
+-- /--
+-- calculate_specific takes as input a pair (e,x), and returns an index to a program which
+-- calculates ψᴼₑ(x) regardless of its input.
+-- -/
+def calculate_specific (ex:ℕ) : ℕ  := comp ex.unpair.1 (Code.const ex.unpair.2)
+@[simp] theorem eval_calculate_specific : eval O (calculate_specific (Nat.pair e x)) _z = eval O e x := by
+  unfold calculate_specific
+  simp? [eval] says simp only [unpair_pair, decodeCode_encodeCode, eval, eval_const, Part.bind_eq_bind, Part.bind_some]
+
+theorem prim_comp₁ : Nat.PrimrecIn O (fun ex => comp ex.unpair.1 ex.unpair.2) := by
+  have h (O:ℕ→ℕ): PrimrecIn₂ O comp := by exact comp_prim
+  exact PrimrecIn.nat_iff.mp (h O)
+  -- unfold PrimrecIn₂ at h
 
 
-@[simp] lemma Nat.RecursiveIn.partCompTotal {O:ℕ→ℕ} {f:ℕ→.ℕ} {g:ℕ→ℕ} (h1: Nat.RecursiveIn O f) (h2: Nat.RecursiveIn O g) : (Nat.RecursiveIn O ↑(f∘g)) := by
-  have h3 : (↑(f∘g):ℕ→.ℕ) = fun x => g x >>= (↑f:ℕ→.ℕ) := by
+-- hm, the proof shouldnt be this long?
+@[simp] theorem prim_calculate_specific : Nat.PrimrecIn O calculate_specific := by
+  have rwmain : calculate_specific = (fun ex:ℕ => (comp ex.unpair.1 ex.unpair.2:ℕ)) ∘ (fun ex:ℕ => Nat.pair ex.unpair.1 (Code.const ex.unpair.2)) := by
+    funext xs
+    simp only [Function.comp_apply, unpair_pair, decodeCode_encodeCode]
+    exact rfl
+  rw [rwmain]
+  have main2 : Nat.PrimrecIn O fun ex:ℕ => Nat.pair ex.unpair.1 (Code.const ex.unpair.2) := by
+    refine PrimrecIn.pair ?_ ?_
+    · exact PrimrecIn.left
+    · have main3 : (fun ex ↦ ((Code.const (unpair ex).2):ℕ)) = (fun ex => (Code.const ex :ℕ)) ∘ fun exa => (unpair exa).2 := by
+        funext xs
+        simp only [Function.comp_apply]
+      have main4 : Nat.PrimrecIn O fun ex => (Code.const ex:ℕ) := by
+        refine PrimrecIn.nat_iff.mp ?_
+        apply const_prim
+      have main5 : Nat.PrimrecIn O fun exa => (unpair exa).2 := by
+        exact PrimrecIn.right
+      rw [main3]
+      apply Nat.PrimrecIn.comp main4 main5
+
+  apply Nat.PrimrecIn.comp prim_comp₁ main2
+
+
+end Nat.RecursiveIn.Code
+
+
+
+
+@[simp] lemma Nat.RecursiveIn.partCompTotal {O:ℕ→ℕ} {f:ℕ→.ℕ} {g:ℕ→ℕ} (h1: Nat.RecursiveIn O f) (h2: Nat.RecursiveIn O g):(Nat.RecursiveIn O ↑(f∘g)) := by
+  have h3:(↑(f∘g):ℕ→.ℕ) = fun x => g x >>= (↑f:ℕ→.ℕ) := by
     funext xs
     simp only [Function.comp_apply, Part.coe_some, Part.bind_eq_bind, Part.bind_some]
   rw [h3]
   exact comp h1 h2
-@[simp] lemma Nat.RecursiveIn.totalComp {O:ℕ→ℕ} {f g:ℕ→ℕ} (h1: Nat.RecursiveIn O f) (h2: Nat.RecursiveIn O g) : (Nat.RecursiveIn O ↑(f∘g)) := by
-  have h3 : (↑(f∘g):ℕ→.ℕ) = fun x => g x >>= (↑f:ℕ→.ℕ) := by
+@[simp] lemma Nat.RecursiveIn.totalComp {O:ℕ→ℕ} {f g:ℕ→ℕ} (h1: Nat.RecursiveIn O f) (h2: Nat.RecursiveIn O g):(Nat.RecursiveIn O ↑(f∘g)) := by
+  have h3:(↑(f∘g):ℕ→.ℕ) = fun x => g x >>= (↑f:ℕ→.ℕ) := by
     funext xs
     simp only [PFun.coe_val, Function.comp_apply, Part.coe_some, Part.bind_eq_bind, Part.bind_some]
   rw [h3]
   exact comp h1 h2
-@[simp] lemma Nat.RecursiveIn.id {O:ℕ→ℕ} : Nat.RecursiveIn O fun x => x := by apply of_primrec Nat.Primrec.id
+@[simp] lemma Nat.RecursiveIn.id {O:ℕ→ℕ}:Nat.RecursiveIn O fun x => x := by apply of_primrec Nat.Primrec.id
 @[simp] lemma Nat.RecursiveIn.someTotal (O:ℕ→ℕ) (f:ℕ→ℕ) (h1: Nat.RecursiveIn O f): Nat.RecursiveIn O fun x => Part.some (f x) := by
   apply Nat.RecursiveIn.totalComp
   · exact h1
@@ -64,8 +104,8 @@ theorem PrimrecIn.PrimrecIn_iff_Primrec : (∀O,Nat.PrimrecIn O f) ↔ Nat.Primr
 @[simp] abbrev Nat.r (n:ℕ) := n.unpair.2
 
 namespace Nat.RecursiveIn.Code
-theorem exists_code_nat {O : ℕ → ℕ} {f : ℕ →. ℕ} : Nat.RecursiveIn O f ↔ ∃ c : ℕ , eval O c = f := by
-  have h {f : ℕ →. ℕ} : Nat.RecursiveIn O f ↔ ∃ c : Nat.RecursiveIn.Code, eval O c = f := by exact
+theorem exists_code_nat {O:ℕ → ℕ} {f:ℕ →. ℕ}:Nat.RecursiveIn O f ↔ ∃ c:ℕ , eval O c = f := by
+  have h {f:ℕ →. ℕ}:Nat.RecursiveIn O f ↔ ∃ c:Nat.RecursiveIn.Code, eval O c = f := by exact
     exists_code
   constructor
   · intro h2
@@ -78,16 +118,16 @@ theorem exists_code_nat {O : ℕ → ℕ} {f : ℕ →. ℕ} : Nat.RecursiveIn O
     have h5: (∃ c:Nat.RecursiveIn.Code, eval O c = f) := by
       use decodeCode c
     exact exists_code.mpr h5
-def eval₁ (O:ℕ→ℕ) : ℕ→.ℕ := fun ex => eval O ex.unpair.1 ex.unpair.2
-def evaln₁ (O:ℕ→ℕ) : ℕ→ℕ := fun abc => Encodable.encode (evaln O abc.r.r abc.l abc.r.l)
-theorem rec_eval₁ : Nat.RecursiveIn O (eval₁ O) := by exact RecursiveIn.nat_iff.mp eval_part
-theorem prim_evaln₁ : Nat.PrimrecIn O (evaln₁ O) := by
+def eval₁ (O:ℕ→ℕ):ℕ→.ℕ := fun ex => eval O ex.unpair.1 ex.unpair.2
+def evaln₁ (O:ℕ→ℕ):ℕ→ℕ := fun abc => Encodable.encode (evaln O abc.r.r abc.l abc.r.l)
+theorem rec_eval₁:Nat.RecursiveIn O (eval₁ O) := by exact RecursiveIn.nat_iff.mp eval_part
+theorem prim_evaln₁:Nat.PrimrecIn O (evaln₁ O) := by
   refine PrimrecIn.nat_iff.mp ?_
   unfold evaln₁
-  have h : (fun (abc : ℕ) ↦ evaln O abc.r.r (abc.l) abc.r.l) = (fun (a:(ℕ×Code)×ℕ) ↦ evaln O a.1.1 a.1.2 a.2) ∘ (fun (abc:ℕ) => ((abc.r.r, abc.l), abc.r.l)) := by
+  have h:(fun (abc:ℕ) ↦ evaln O abc.r.r (abc.l) abc.r.l) = (fun (a:(ℕ×Code)×ℕ) ↦ evaln O a.1.1 a.1.2 a.2) ∘ (fun (abc:ℕ) => ((abc.r.r, abc.l), abc.r.l)) := by
     exact rfl
   -- rw [h]
-  have h2 : PrimrecIn O (fun (abc:ℕ) =>    (((abc.r.r, abc.l), abc.r.l):(ℕ×Code)×ℕ)    ) := by
+  have h2:PrimrecIn O (fun (abc:ℕ) =>    (((abc.r.r, abc.l), abc.r.l):(ℕ×Code)×ℕ)    ) := by
     refine _root_.PrimrecIn.pair ?_ ?_
     · apply _root_.PrimrecIn.pair (_root_.PrimrecIn.comp (PrimrecIn.nat_iff.mpr PrimrecIn.right) (PrimrecIn.nat_iff.mpr PrimrecIn.right))
       apply _root_.PrimrecIn.comp
@@ -97,16 +137,16 @@ theorem prim_evaln₁ : Nat.PrimrecIn O (evaln₁ O) := by
   apply _root_.PrimrecIn.comp evaln_prim h2
 
 
-theorem exists_code_for_eval₁ : ∃ c:ℕ, eval O c = eval₁ O := by
+theorem exists_code_for_eval₁:∃ c:ℕ, eval O c = eval₁ O := by
   apply (exists_code_nat.mp)
   exact rec_eval₁
 
-theorem Nat.RecursiveIn.evalRecInO' {O} {f:ℕ→.ℕ} (h:Nat.RecursiveIn O f) : Nat.RecursiveIn O (fun x => (f x) >>= (eval₁ O)) := by
+theorem Nat.RecursiveIn.evalRecInO' {O} {f:ℕ→.ℕ} (h:Nat.RecursiveIn O f):Nat.RecursiveIn O (fun x => (f x) >>= (eval₁ O)) := by
   simp only [Part.bind_eq_bind]
   refine _root_.Nat.RecursiveIn.comp ?_ h
   apply rec_eval₁
-theorem Nat.RecursiveIn.eval_K_computable : Nat.RecursiveIn O (fun x ↦ eval O x x) := by
-  have h : (fun (x:ℕ) ↦ eval O x x) = (fun (x:ℕ) => eval O x.unpair.1 x.unpair.2) ∘ (fun x=>Nat.pair x x) := by
+theorem Nat.RecursiveIn.eval_K_computable:Nat.RecursiveIn O (fun x ↦ eval O x x) := by
+  have h:(fun (x:ℕ) ↦ eval O x x) = (fun (x:ℕ) => eval O x.unpair.1 x.unpair.2) ∘ (fun x=>Nat.pair x x) := by
     funext xs
     simp only [Function.comp_apply, Nat.unpair_pair]
   rw [h]
@@ -122,18 +162,18 @@ end Nat.RecursiveIn.Code
 
 
 namespace Nat.RecursiveIn.Code
--- inductive code_prim : ℕ → Prop
--- inductive code_prim : Code → Type
-inductive code_prim : Code → Prop
-| zero : code_prim zero
-| succ : code_prim succ
-| left : code_prim left
-| right : code_prim right
-| oracle : code_prim oracle
-| pair {a b:Code} (ha:code_prim a) (hb:code_prim b) : code_prim (pair a b)
-| comp {a b:Code} (ha:code_prim a) (hb:code_prim b) : code_prim (comp a b)
-| prec {a b:Code} (ha:code_prim a) (hb:code_prim b) : code_prim (prec a b)
-theorem prim_total (h:code_prim c) : ∀x,(eval O c x).Dom := by
+-- inductive code_prim:ℕ → Prop
+-- inductive code_prim:Code → Type
+inductive code_prim:Code → Prop
+| zero:code_prim zero
+| succ:code_prim succ
+| left:code_prim left
+| right:code_prim right
+| oracle:code_prim oracle
+| pair {a b:Code} (ha:code_prim a) (hb:code_prim b):code_prim (pair a b)
+| comp {a b:Code} (ha:code_prim a) (hb:code_prim b):code_prim (comp a b)
+| prec {a b:Code} (ha:code_prim a) (hb:code_prim b):code_prim (prec a b)
+theorem prim_total (h:code_prim c):∀x,(eval O c x).Dom := by
   induction h with
   | zero                   => simp [eval]; exact fun x ↦ trivial
   | succ                   => simp [eval];
@@ -159,14 +199,14 @@ theorem prim_total (h:code_prim c) : ∀x,(eval O c x).Dom := by
       use IH'
       apply hb_ih
 
-def eval_total (O:ℕ→ℕ) (c:Code) {h:∀x,(eval O c x).Dom} : ℕ→ℕ := fun x => (eval O c x).get (h x)
--- def eval_prim (O:ℕ→ℕ) (c:Code) {h:code_prim c} : ℕ→ℕ := fun x => (eval O c x).get (prim_total h x)
--- def eval_prim (O:ℕ→ℕ) (h:code_prim c) : ℕ→ℕ :=
+def eval_total (O:ℕ→ℕ) (c:Code) {h:∀x,(eval O c x).Dom}:ℕ→ℕ := fun x => (eval O c x).get (h x)
+-- def eval_prim (O:ℕ→ℕ) (c:Code) {h:code_prim c}:ℕ→ℕ := fun x => (eval O c x).get (prim_total h x)
+-- def eval_prim (O:ℕ→ℕ) (h:code_prim c):ℕ→ℕ :=
 -- match h with
 
 #check code_prim.zero
 #check zero.code_prim
--- def eval_prim (O:ℕ→ℕ) : (code_prim c)→ℕ→ℕ
+-- def eval_prim (O:ℕ→ℕ):(code_prim c)→ℕ→ℕ
 -- | code_prim.zero       => fun x=>0
 -- | code_prim.succ       => Nat.succ
 -- | code_prim.left       => Nat.l
@@ -176,7 +216,7 @@ def eval_total (O:ℕ→ℕ) (c:Code) {h:∀x,(eval O c x).Dom} : ℕ→ℕ := f
 -- | code_prim.comp cf cg => fun n => eval_prim O cf (eval_prim O cg n)
 -- | code_prim.prec cf cg => unpaired fun z n => n.rec (eval_prim O cf z) fun y IH => (eval_prim O cg) <| pair z <| pair y IH
 -- | _ => 0
-def eval_prim (O:ℕ→ℕ) : Code→ℕ→ℕ
+def eval_prim (O:ℕ→ℕ):Code→ℕ→ℕ
 | zero       => fun x=>0
 | succ       => Nat.succ
 | left       => Nat.l
@@ -188,8 +228,8 @@ def eval_prim (O:ℕ→ℕ) : Code→ℕ→ℕ
 | rfind' _ => 0
 
 
--- theorem eval_prim_eq_eval (h:code_prim c) : eval_prim O h = eval O c := by
-theorem eval_prim_eq_eval (h:code_prim c) : eval_prim O c = eval O c := by
+-- theorem eval_prim_eq_eval (h:code_prim c):eval_prim O h = eval O c := by
+theorem eval_prim_eq_eval (h:code_prim c):eval_prim O c = eval O c := by
   induction h with
   | zero => exact rfl
   | succ => exact rfl
@@ -213,7 +253,7 @@ theorem eval_prim_eq_eval (h:code_prim c) : eval_prim O c = eval O c := by
     funext xs
     simp
     expose_names
-    -- have h0 : eval O b xs = Part.some (eval_prim O b xs) := by exact congrFun (_root_.id (Eq.symm hb_ih)) xs
+    -- have h0:eval O b xs = Part.some (eval_prim O b xs) := by exact congrFun (_root_.id (Eq.symm hb_ih)) xs
     -- simp [h0]
     simp only [show eval O b xs = Part.some (eval_prim O b xs) from by exact congrFun (_root_.id (Eq.symm hb_ih)) xs]
     simp
@@ -231,7 +271,7 @@ theorem eval_prim_eq_eval (h:code_prim c) : eval_prim O c = eval O c := by
       simp
       simp only [show eval O a (unpair xs).1 = Part.some (eval_prim O a (unpair xs).1) from by exact congrFun (_root_.id (Eq.symm ha_ih)) (unpair xs).1]
     | succ y' IH' =>
-      have h0 : @Nat.rec (fun x ↦ Part ℕ) (eval O a (unpair xs).1) (fun y IH ↦ IH.bind fun i ↦ eval O b (Nat.pair (unpair xs).1 (Nat.pair y i))) (y' + 1) = ((@Nat.rec (fun x ↦ Part ℕ) (eval O a (unpair xs).1)
+      have h0:@Nat.rec (fun x ↦ Part ℕ) (eval O a (unpair xs).1) (fun y IH ↦ IH.bind fun i ↦ eval O b (Nat.pair (unpair xs).1 (Nat.pair y i))) (y' + 1) = ((@Nat.rec (fun x ↦ Part ℕ) (eval O a (unpair xs).1)
   (fun y IH ↦ IH.bind fun i ↦ eval O b (Nat.pair (unpair xs).1 (Nat.pair y i))) y').bind fun i ↦ eval O b (Nat.pair (unpair xs).1 (Nat.pair y' i))) := by
         exact rfl
       rw [h0]
@@ -249,7 +289,7 @@ theorem eval_prim_eq_eval (h:code_prim c) : eval_prim O c = eval O c := by
 
 
 
-theorem code_prim_prop (h:code_prim c) : ∀ O, Nat.PrimrecIn O (eval_prim O c) := by
+theorem code_prim_prop (h:code_prim c):∀ O, Nat.PrimrecIn O (eval_prim O c) := by
   induction h with
   | zero => unfold eval_prim; exact fun O ↦ PrimrecIn.zero
   | succ => unfold eval_prim; exact fun O ↦ PrimrecIn.succ
@@ -269,7 +309,7 @@ end Nat.RecursiveIn.Code
 /-- Maps zero to 1 and non-zero natural numbers to 0. This is the inverse of `Nat.sg` for boolean-like computations. -/
 @[simp] def Nat.sg' := fun x => if x=0 then 1 else 0
 
-theorem Nat.Primrec.sg' : Nat.Primrec Nat.sg' := by
+theorem Nat.Primrec.sg':Nat.Primrec Nat.sg' := by
   let construction := comp (prec (const 1) (((zero).comp left).comp left)) (pair zero .id)
   apply Nat.Primrec.of_eq construction
   simp only [unpaired, id_eq, unpair_pair, Nat.sg']
@@ -279,7 +319,7 @@ theorem Nat.Primrec.sg' : Nat.Primrec Nat.sg' := by
   | succ n _ => simp only [Nat.add_eq_zero, one_ne_zero, and_false, ↓reduceIte]
 
 open Nat.Primrec in private def sg_construction := comp (prec zero (((const 1).comp left).comp left)) (pair zero .id)
--- private theorem sg_construction_prop : sg_construction=Nat.sg :=
+-- private theorem sg_construction_prop:sg_construction=Nat.sg :=
 
 -- I want to have a single construction, a single proof that that construction is equivalent to some function, and from that
 -- show that the function 1. has a code and is 2. primrec/rec.
@@ -289,7 +329,7 @@ open Nat.Primrec in private def sg_construction := comp (prec zero (((const 1).c
 
 namespace Nat.RecursiveIn.Code
 
-theorem const_prim2 : ∀ n, code_prim (Code.const n) := by
+theorem const_prim2:∀ n, code_prim (Code.const n) := by
   intro n
   induction n
   · unfold Code.const; exact code_prim.zero
@@ -297,16 +337,16 @@ theorem const_prim2 : ∀ n, code_prim (Code.const n) := by
     expose_names
     exact code_prim.comp code_prim.succ h
 
-@[simp] theorem const_eval : ∀ n m, eval_prim O (Code.const n) m = n
+@[simp] theorem const_eval:∀ n m, eval_prim O (Code.const n) m = n
   | 0, _ => rfl
   | n + 1, m => by simp! [const_eval n m]
-@[simp] theorem id_eval (n) : eval_prim O Code.id n = n := by simp! [Seq.seq, Code.id]
+@[simp] theorem id_eval (n):eval_prim O Code.id n = n := by simp! [Seq.seq, Code.id]
 end Nat.RecursiveIn.Code
 
 namespace Nat.RecursiveIn.Code
 def code_sg := comp (prec zero (((Code.const 1).comp left).comp left)) (pair zero .id)
-theorem code_sg_prim : code_prim code_sg := by unfold code_sg; repeat constructor
-theorem code_sg_prop : eval_prim O code_sg = Nat.sg := by
+theorem code_sg_prim:code_prim code_sg := by unfold code_sg; repeat constructor
+theorem code_sg_prop:eval_prim O code_sg = Nat.sg := by
   simp [code_sg]
   simp [eval_prim]
   funext n
@@ -315,8 +355,8 @@ theorem code_sg_prop : eval_prim O code_sg = Nat.sg := by
   | succ n _ => simp
 end Nat.RecursiveIn.Code
 
-theorem Nat.PrimrecIn.sg : Nat.PrimrecIn O Nat.sg := by rw [←code_sg_prop]; apply code_prim_prop code_sg_prim
-theorem Nat.Primrec.sg : Nat.Primrec Nat.sg := by exact PrimrecIn.PrimrecIn_Empty PrimrecIn.sg
+theorem Nat.PrimrecIn.sg:Nat.PrimrecIn O Nat.sg := by rw [←code_sg_prop]; apply code_prim_prop code_sg_prim
+theorem Nat.Primrec.sg:Nat.Primrec Nat.sg := by exact PrimrecIn.PrimrecIn_Empty PrimrecIn.sg
 
 
   -- let construction := comp (prec zero (((const 1).comp left).comp left)) (pair zero .id)
@@ -331,13 +371,13 @@ theorem Nat.Primrec.sg : Nat.Primrec Nat.sg := by exact PrimrecIn.PrimrecIn_Empt
 
 
 
-@[simp] lemma Nat.RecursiveIn.pair' (f g : ℕ→ℕ) : ((↑fun x ↦ Nat.pair (f x) (g x)):ℕ→.ℕ)= fun (x:ℕ) => (Nat.pair <$> (f x) <*> (g x)) := by
+@[simp] lemma Nat.RecursiveIn.pair' (f g:ℕ→ℕ):((↑fun x ↦ Nat.pair (f x) (g x)):ℕ→.ℕ)= fun (x:ℕ) => (Nat.pair <$> (f x) <*> (g x)) := by
   simp [Seq.seq]
   funext xs
   simp only [PFun.coe_val]
 @[simp] lemma Nat.RecursiveIn.totalComp' {O:ℕ→ℕ} {f g:ℕ→ℕ} (hf: Nat.RecursiveIn O f) (hg: Nat.RecursiveIn O g): (Nat.RecursiveIn O (fun x => (f (g x)):ℕ→ℕ) ) := by apply Nat.RecursiveIn.totalComp (hf) (hg)
 @[simp] lemma Nat.RecursiveIn.comp₂ {O:ℕ→ℕ} {f:ℕ→ℕ→.ℕ} {g h:ℕ→ℕ} (hf: Nat.RecursiveIn O fun x => f x.unpair.1 x.unpair.2) (hg: Nat.RecursiveIn O g) (hh: Nat.RecursiveIn O h): (Nat.RecursiveIn O (fun x => (f (g x) (h x))) ) := by
-  have main : (fun x => (f (g x) (h x))) = ((fun x => f x.unpair.1 x.unpair.2) ∘ (fun n ↦ Nat.pair (g n) (h n))) := by
+  have main:(fun x => (f (g x) (h x))) = ((fun x => f x.unpair.1 x.unpair.2) ∘ (fun n ↦ Nat.pair (g n) (h n))) := by
     funext xs
     simp only [Function.comp_apply, unpair_pair]
   rw [main]
@@ -345,7 +385,7 @@ theorem Nat.Primrec.sg : Nat.Primrec Nat.sg := by exact PrimrecIn.PrimrecIn_Empt
   · rw [Nat.RecursiveIn.pair']
     apply Nat.RecursiveIn.pair hg hh
 @[simp] lemma Nat.RecursiveIn.totalComp₂ {O:ℕ→ℕ} {f:ℕ→ℕ→ℕ} {g h:ℕ→ℕ} (hf: Nat.RecursiveIn O fun x => f x.unpair.1 x.unpair.2) (hg: Nat.RecursiveIn O g) (hh: Nat.RecursiveIn O h): (Nat.RecursiveIn O (fun x => (f (g x) (h x)):ℕ→ℕ) ) := by
-  have main : (fun x => (f (g x) (h x)):ℕ→ℕ) = ((fun x => f x.unpair.1 x.unpair.2) ∘ (fun n ↦ Nat.pair (g n) (h n))) := by
+  have main:(fun x => (f (g x) (h x)):ℕ→ℕ) = ((fun x => f x.unpair.1 x.unpair.2) ∘ (fun n ↦ Nat.pair (g n) (h n))) := by
     funext xs
     simp only [Function.comp_apply, Nat.unpair_pair]
   rw [main]
@@ -354,12 +394,12 @@ theorem Nat.Primrec.sg : Nat.Primrec Nat.sg := by exact PrimrecIn.PrimrecIn_Empt
   · rw [Nat.RecursiveIn.pair']
     apply Nat.RecursiveIn.pair hg hh
 
-theorem Nat.RecursiveIn.ifz1 {O:ℕ→ℕ} {c:ℕ→ℕ} (hc : Nat.RecursiveIn O c): Nat.RecursiveIn O (fun x => if (c x=0) then (a:ℕ) else (b:ℕ) : ℕ→ℕ) := by
+theorem Nat.RecursiveIn.ifz1 {O:ℕ→ℕ} {c:ℕ→ℕ} (hc:Nat.RecursiveIn O c): Nat.RecursiveIn O (fun x => if (c x=0) then (a:ℕ) else (b:ℕ):ℕ→ℕ) := by
   let construction := fun x =>
     Nat.add
     (Nat.mul b (Nat.sg (c x)))
     (Nat.mul a (Nat.sg' (c x)))
-  have consRecin : Nat.RecursiveIn O construction := by
+  have consRecin:Nat.RecursiveIn O construction := by
     simp only [construction]
     apply Nat.RecursiveIn.totalComp₂
     · apply of_primrec Nat.Primrec.add
@@ -375,7 +415,7 @@ theorem Nat.RecursiveIn.ifz1 {O:ℕ→ℕ} {c:ℕ→ℕ} (hc : Nat.RecursiveIn O
       · apply Nat.RecursiveIn.totalComp'
         · exact of_primrec Nat.Primrec.sg'
         · exact hc
-  have consEq: (fun x => if (c x=0) then (a:ℕ) else (b:ℕ) : ℕ→ℕ) = construction := by
+  have consEq: (fun x => if (c x=0) then (a:ℕ) else (b:ℕ):ℕ→ℕ) = construction := by
     simp [construction]
     funext xs
     cases Classical.em (c xs = 0) with -- do i really need classical.em here?
@@ -389,11 +429,11 @@ theorem Nat.RecursiveIn.ifz1 {O:ℕ→ℕ} {c:ℕ→ℕ} (hc : Nat.RecursiveIn O
 
 
 
-theorem Primrec.projection {f : α → β → σ} {a:α} (h:Primrec₂ f) : Primrec (f a) := by
+theorem Primrec.projection {f:α → β → σ} {a:α} (h:Primrec₂ f):Primrec (f a) := by
   refine Primrec₂.comp h ?_ ?_
   · exact const a
   · exact Primrec.id
-lemma Nat.Primrec.pair_proj : Nat.Primrec (Nat.pair x) := by
+lemma Nat.Primrec.pair_proj:Nat.Primrec (Nat.pair x) := by
   refine Primrec.nat_iff.mp ?_
   apply Primrec.projection
   exact Primrec₂.natPair
@@ -401,13 +441,13 @@ lemma Nat.Primrec.pair_proj : Nat.Primrec (Nat.pair x) := by
 
 
 
-theorem Nat.RecursiveIn.ite {O:ℕ→ℕ} {f g : ℕ→.ℕ} {c:ℕ→ℕ} (hc : Nat.RecursiveIn O c) (hf : Nat.RecursiveIn O f) (hg : Nat.RecursiveIn O g) : Nat.RecursiveIn O fun a => if (c a=0) then (f a) else (g a) := by
-    have exists_index_for_f : ∃ c : ℕ, eval O c = f := by exact exists_code_nat.mp hf
-    have exists_index_for_g : ∃ c : ℕ, eval O c = g := by exact exists_code_nat.mp hg
+theorem Nat.RecursiveIn.ite {O:ℕ→ℕ} {f g:ℕ→.ℕ} {c:ℕ→ℕ} (hc:Nat.RecursiveIn O c) (hf:Nat.RecursiveIn O f) (hg:Nat.RecursiveIn O g):Nat.RecursiveIn O fun a => if (c a=0) then (f a) else (g a) := by
+    have exists_index_for_f:∃ c:ℕ, eval O c = f := by exact exists_code_nat.mp hf
+    have exists_index_for_g:∃ c:ℕ, eval O c = g := by exact exists_code_nat.mp hg
     rcases exists_index_for_f with ⟨index_f,index_f_is_f⟩
     rcases exists_index_for_g with ⟨index_g,index_g_is_g⟩
 
-    have main2 : (fun a => if (c a=0) then (f a) else (g a)) = fun a => Nat.pair (if c a=0 then (index_f) else (index_g)) a >>= eval₁ O := by
+    have main2:(fun a => if (c a=0) then (f a) else (g a)) = fun a => Nat.pair (if c a=0 then (index_f) else (index_g)) a >>= eval₁ O := by
       funext xs
       cases Classical.em (c xs = 0) with
       | inl h =>
@@ -433,7 +473,7 @@ theorem Nat.RecursiveIn.ite {O:ℕ→ℕ} {f g : ℕ→.ℕ} {c:ℕ→ℕ} (hc :
 -- for code_ifeq
 
 open Nat.Primrec in
-theorem Nat.Primrec.dist : Nat.Primrec (unpaired Nat.dist) := by
+theorem Nat.Primrec.dist:Nat.Primrec (unpaired Nat.dist) := by
   let construction := comp Nat.Primrec.add (Nat.Primrec.pair Nat.Primrec.sub (Nat.Primrec.swap' Nat.Primrec.sub))
   apply Nat.Primrec.of_eq construction
   simp
@@ -441,5 +481,5 @@ theorem Nat.Primrec.dist : Nat.Primrec (unpaired Nat.dist) := by
   exact fun n ↦ rfl
 
 /--`[code_if_eval_eq c](x)=0 if x.1=x.2 else 1`-/
-def code_if_eq : ℕ→ℕ := fun x => 0
-theorem code_if_eq_prop : eval O (code_if_eq e) ab = if (Nat.succ ab.l.r=eval O e (Nat.pair ab.l.l ab.r)) then 0 else 1 := by sorry
+def code_if_eq:ℕ→ℕ := fun x => 0
+theorem code_if_eq_prop:eval O (code_if_eq e) ab = if (Nat.succ ab.l.r=eval O e (Nat.pair ab.l.l ab.r)) then 0 else 1 := by sorry
