Computability/Basic.lean
@@ -1,0 +1,66 @@
+import Computability.Oracle
+
+@[simp] abbrev TuringReducible (f g : ℕ → ℕ) : Prop := Nat.RecursiveIn g f
+@[simp] abbrev TuringReducibleStrict (f g : ℕ → ℕ) : Prop := Nat.RecursiveIn g f ∧ ¬ Nat.RecursiveIn f g
+@[simp] abbrev TuringEquivalent (f g : ℕ → ℕ) : Prop := AntisymmRel TuringReducible f g
+
+@[reducible,simp,inherit_doc] scoped[Computability] infix:50 " ≤ᵀᶠ " => TuringReducible
+@[reducible,simp,inherit_doc] scoped[Computability] infix:50 " ≡ᵀᶠ " => TuringEquivalent
+@[reducible,simp,inherit_doc] scoped[Computability] infix:50 " <ᵀᶠ " => TuringReducibleStrict
+
+open scoped Computability
+
+protected theorem TuringReducible.refl (f : ℕ → ℕ) : f ≤ᵀᶠ f := by exact Nat.RecursiveIn.oracle
+protected theorem TuringReducible.rfl : f ≤ᵀᶠ f := .refl _
+
+instance : IsRefl (ℕ → ℕ) TuringReducible where refl _ := .rfl
+
+theorem TuringReducible.trans (hg : f ≤ᵀᶠ g) (hh : g ≤ᵀᶠ h) : f ≤ᵀᶠ h := by
+  generalize z : (↑f:ℕ→.ℕ)=x at hg
+  simp only [TuringReducible,z] at *
+  induction hg with
+  | zero => exact Nat.RecursiveIn.zero
+  | succ => exact Nat.RecursiveIn.succ
+  | left => exact Nat.RecursiveIn.left
+  | right => exact Nat.RecursiveIn.right
+  | oracle => exact hh
+  | pair hf hh hf_ih hh_ih => (expose_names; exact Nat.RecursiveIn.pair hf_ih hh_ih)
+  | comp hf hh hf_ih hh_ih => (expose_names; exact Nat.RecursiveIn.comp hf_ih hh_ih)
+  | prec hf hh hf_ih hh_ih => (expose_names; exact Nat.RecursiveIn.prec hf_ih hh_ih)
+  | rfind hf ih => (expose_names; exact Nat.RecursiveIn.rfind ih)
+
+theorem TuringReducible.trans' (hg : Nat.RecursiveIn g f) (hh : g ≤ᵀᶠ h) : Nat.RecursiveIn h f := by
+  generalize z : (↑f:ℕ→.ℕ)=x at hg
+  simp only [TuringReducible,z] at *
+  induction hg with
+  | zero => exact Nat.RecursiveIn.zero
+  | succ => exact Nat.RecursiveIn.succ
+  | left => exact Nat.RecursiveIn.left
+  | right => exact Nat.RecursiveIn.right
+  | oracle => exact hh
+  | pair hf hh hf_ih hh_ih => (expose_names; exact Nat.RecursiveIn.pair hf_ih hh_ih)
+  | comp hf hh hf_ih hh_ih => (expose_names; exact Nat.RecursiveIn.comp hf_ih hh_ih)
+  | prec hf hh hf_ih hh_ih => (expose_names; exact Nat.RecursiveIn.prec hf_ih hh_ih)
+  | rfind hf ih => (expose_names; exact Nat.RecursiveIn.rfind ih)
+
+instance : IsTrans (ℕ→ℕ) TuringReducible := ⟨@TuringReducible.trans⟩
+instance : IsPreorder (ℕ→ℕ) TuringReducible where refl := .refl
+theorem TuringEquivalent.equivalence : Equivalence TuringEquivalent := (AntisymmRel.setoid _ _).iseqv
+@[refl] protected theorem TuringEquivalent.refl (f : ℕ→ℕ) : f ≡ᵀᶠ f := Equivalence.refl equivalence f
+@[symm] theorem TuringEquivalent.symm {f g : ℕ→ℕ} (h : f ≡ᵀᶠ g) : g ≡ᵀᶠ f := Equivalence.symm equivalence h
+@[trans] theorem TuringEquivalent.trans (f g h : ℕ→ℕ) (h₁ : f ≡ᵀᶠ g) (h₂ : g ≡ᵀᶠ h) : f ≡ᵀᶠ h := Equivalence.trans equivalence h₁ h₂
+
+/--
+Instance declaring that `Nat.RecursiveIn` is a preorder.
+-/
+instance : IsPreorder (ℕ→ℕ) TuringReducible where
+  refl := TuringReducible.refl
+  trans := @TuringReducible.trans
+
+abbrev FuncTuringDegree :=
+  Antisymmetrization _ TuringReducible
+private instance : Preorder (ℕ→ℕ) where
+  le := TuringReducible
+  le_refl := .refl
+  le_trans _ _ _ := TuringReducible.trans
+  lt := TuringReducibleStrict
